Support for call instruction

examples/sgx/Ast.fst
@@ -22,6 +22,8 @@ type stmt =
  |Cmp of u64 * exp * exp * exp
  |Store of u64 * u64*exp * exp
  |Assign of  u64 * exp * exp
+ |Push of  u64 * exp 
+ |Pop of u64 * exp 
  |Load of u64 *exp * u64* exp
  |Seq of u64 * (list stmt)
  |If of  u64 * exp * stmt * stmt
@@ -34,3 +36,17 @@ type stmt =
 type lambda = string * stmt
 type program = list lambda
 
+type accesstype =
+| Public
+| Private
+
+type argument =
+| Mkintarg 
+| Mkstringarg
+ 
+(* 0x1000  foo [int;int..] public  *)
+type callentry =
+ | MkCallentry : address -> string -> (list argument) -> accesstype -> callentry
+
+type calltable =
+ | MkCalltable : (list callentry) -> calltable 
