examples/sgx/SGXState.fst
@@ -15,5 +15,4 @@ val get_reg_list: cpuregstate -> Tot (list register)
 let get_reg_list = function
  |Mkcpuregstate li -> li
 
- 
 
