examples/sgx/Test.fst
@@ -1,18 +1,90 @@
 module Test
 open Ast
 
-  (* let mylambda = ("main", [(Store(1uL,(Register "rax"),(Register "rcx")))])  *)
+(*
+  let mylambda = [("main", Seq (1200uL, [(Assign (1200uL, (Register "rbx"), (Constant 1400uL)))]))]
+  let mylambda = [("main", Seq (1200uL, [(Assign (1200uL, (Register "rbx"), (Constant 1400uL)));(Store (1201uL, 1uL, (Register "rbx"), (Constant 10uL)))]))]
+ *)
 
  (*
+ main:
+  rbp := rsp
   rbx := 1400uL
   store rbx 10uL 
-  rcx := load(rbx)
-  rax := 0
- L: add rax 1
-    jump L
-    return
-  let mylambda = ("main", Seq (1200uL, [(Assign (1200uL, (Register "rbx"), (Constant 1400uL)))]))
-  let mylambda = ("main", Seq (1200uL, [(Assign (1200uL, (Register "rbx"), (Constant 1400uL)));(Store (1201uL, 1uL, (Register "rbx"), (Constant 10uL)))]))
+  rdx := load(rbx)
+  rcx := 0
+  call "foo"
+  rsp := rbp
+  return
+
+ counter:
+    rbp := rsp
+ L1: add rcx rcx 1
+    cmp flag rdx rcx
+    if flag = 1 then 
+      rax := rcx
+      jump L2 
+   else
+      jump L1
+ L2: rsp := rbp
+     return 
   *)
-  let mylambda = ("main", Seq (1200uL, [(Assign (1200uL, (Register "rbx"), (Constant 1400uL)));(Store (1201uL, 1uL, (Register "rbx"), (Constant 10uL)));(Load (1202uL, (Register "rcx"), 1uL, (Register "rbx")));(Assign (1203uL, (Register "rax"), (Constant 0uL)));(Add (1204uL, (Register "rax"), (Register "rax"), (Constant 1uL)));(Jump (1205uL, Constant 1204uL)); (Return 1206uL)])) 
-  let testprogram = [mylambda] 
+
+  let mylambda = [
+		 ("main", 
+		 Seq (1200uL, [ 
+				
+				(Assign (1200uL, (Register "rbp"), (Register "rsp")));
+				(Call (1201uL, (Constant 1210uL)));
+				(Return 1204uL)
+				]));
+		("counter", 
+		 Seq (1210uL, [ (Push (1210uL, (Register "rbp")));
+				(Pop (1211uL, (Register "rax")));
+				(Return 1212uL)
+				]))
+		]
+  (*
+  let mylambda = [
+		 ("main", 
+		 Seq (1200uL, [(Assign (1200uL, (Register "rbp"), (Constant 1000uL)));(Push (1200uL, (Register "rbp")));
+				(Assign (1201uL, (Register "rbp"), (Register "rsp")));
+				(Assign (1202uL, (Register "rbx"), (Constant 1402uL)));
+		 		(Store (1203uL, 1uL, (Register "rbx"), (Constant 10uL)));
+				(Load (1204uL, (Register "rdx"), 1uL, (Register "rbx")));
+				(Call (1205uL, (Constant 1210uL)));
+		 		(Assign (1206uL, (Register "rsp"), (Register "rbp")));
+				(Pop (1207uL, (Register "rbp")));
+				(Return 1208uL)	
+				]));
+		("counter", 
+		 Seq (1210uL, [(Push (1210uL, (Register "rbp")));
+				(Assign (1211uL, (Register "rbp"), (Register "rsp")));
+				(Add (1212uL, (Register "rcx"), (Register "rcx"),(Constant 1uL)));
+				(Cmp (1213uL, (Register "flag"), (Register "rdx"),(Register "rcx")));
+		 		(If (1214uL, (Register "flag"), Seq (1215uL, [  
+						(Assign (1215uL, (Register "rax"), (Register "rcx")));
+						(Jump (1216uL, (Constant 1218uL) ))
+						 ]),
+					     Seq (1217uL, [  
+						(Jump (1217uL, (Constant 1212uL) ))
+						 ])
+				    )
+				);
+		 		(Assign (1218uL, (Register "rsp"), (Register "rbp")));
+				(Pop (1219uL, (Register "rbp")));
+				(Return 1220uL)
+				]))
+		]
+*)
+let testprogram = mylambda 
+let make_callentry = [(MkCallentry 1200uL "main" [] Public);(MkCallentry 1210uL "counter" [Mkintarg;Mkintarg] Public)]
+let make_calltable = 
+		   let calltabentry = make_callentry in
+			(MkCalltable calltabentry)
+
+ (* Place holder for parsing manifest and getting the start addresses and  
+    calltable. For now just making calltable
+ *)
+let parse_manifest _ = make_calltable
+
